.

GIT.v
@@ -9,6 +9,117 @@ Import ListNotations.
 
 Section Preliminaries.
 
+Lemma div_mod_uniqueness :
+  forall a : nat,
+  forall b : nat,
+  forall q : nat,
+  forall r : nat,
+  a = b * q + r ->
+  r < b ->
+  a / b = q /\ a mod b = r.
+Proof.
+  assert (forall x : nat, forall y : nat, x > y <-> (exists z : nat, x = S (y + z))).
+  { intros x y; constructor.
+    - intros H; induction H.
+      + exists 0; lia.
+      + destruct IHle as [z H0]; exists (S z); lia.
+    - intros H; destruct H as [z H]; lia.
+  }
+  intros a b q r H1 H2.
+  assert (H0 : a = b * (a / b) + (a mod b)) by (apply (Nat.div_mod a b); lia).
+  assert (H3 : 0 <= a mod b < b).
+  { apply (Nat.mod_bound_pos a b).
+    - lia.
+    - lia.
+  }
+  assert (H4 : ~ q > a / b).
+  { intros H4.
+    assert (H5 : exists z : nat, q = S (a / b + z)) by (apply (H q (a / b)); lia).
+    destruct H5 as [z H5].
+    cut (b * q + r >= b * S (a / b) + r); lia.
+  }
+  assert (H5 : ~ q < a / b).
+  { intros H5.
+    assert (H6 : exists z : nat, a / b = S (q + z)) by (apply (H (a / b) q); lia).
+    destruct H6 as [z H6].
+    cut (b * q + a mod b >= b * S (a / b) + a mod b); lia.
+  }
+  assert (H6 : q = a / b) by lia; assert (H7 : r = a mod b) by lia; lia.
+Qed.
+
+Fixpoint sum_from_0_to (n : nat) : nat :=
+  match n with
+  | 0 => 0
+  | S n' => n + sum_from_0_to n'
+  end
+.
+
+Theorem sum_from_0_to_is :
+  forall n : nat,
+  2 * sum_from_0_to n = n * (S n).
+Proof.
+  intros n; induction n.
+  - intuition.
+  - simpl in *; lia.
+Qed.
+
+Fixpoint cantor_pairing (n : nat) : nat * nat :=
+  match n with
+  | 0 => (0, 0)
+  | S n' =>
+    match cantor_pairing n' with
+    | (0, y) => (S y, 0)
+    | (S x, y) => (x, S y)
+    end
+  end
+.
+
+Lemma cantor_pairing_is_surjective :
+  forall x : nat,
+  forall y : nat,
+  (x, y) = cantor_pairing (sum_from_0_to (x + y) + y).
+Proof.
+  cut (forall z : nat, forall y : nat, forall x : nat, z = x + y -> (x, y) = cantor_pairing (sum_from_0_to z + y)); eauto.
+  intros z; induction z.
+  - intros y x H; assert (H0 : x = 0) by lia; assert (H1 : y = 0) by lia; subst; eauto.
+  - intros y; induction y.
+    + intros x H.
+      assert (H0 : x = S z) by lia.
+      subst; simpl cantor_pairing; destruct (cantor_pairing (z + sum_from_0_to z + 0)) eqn: H0.
+      assert (H1 : (0, z) = cantor_pairing (sum_from_0_to z + z)) by (apply IHz; reflexivity).
+      rewrite Nat.add_0_r in H0; rewrite Nat.add_comm in H0; rewrite H0 in H1.
+      inversion H1; subst; reflexivity.
+    + intros x H.
+      assert (H0 : (S x, y) = cantor_pairing (sum_from_0_to (S z) + y)) by (apply (IHy (S x)); lia).
+      assert (H1 : z + sum_from_0_to z + S y = sum_from_0_to (S z) + y) by (simpl; lia).
+      simpl; rewrite H1; rewrite <- H0; eauto.
+Qed.
+
+Lemma cantor_pairing_is_injective :
+  forall n : nat,
+  forall x : nat,
+  forall y : nat,
+  cantor_pairing n = (x, y) ->
+  n = sum_from_0_to (x + y) + y.
+Proof.
+  intros n; induction n.
+  - simpl; intros x y H; inversion H; subst; reflexivity.
+  - simpl; intros x y H; destruct (cantor_pairing n) as [x' y'] eqn: H0; destruct x'.
+    + inversion H; subst; repeat (rewrite Nat.add_0_r); simpl; rewrite (IHn 0 y' eq_refl); rewrite Nat.add_0_l; lia.
+    + inversion H; subst; rewrite (IHn (S x) y' eq_refl); assert (H1 : forall x' : nat, S x' + y' = x' + S y') by lia; repeat (rewrite H1); lia.
+Qed.
+
+Theorem cantor_pairing_is :
+  forall n : nat,
+  forall x : nat,
+  forall y : nat,
+  cantor_pairing n = (x, y) <-> n = sum_from_0_to (x + y) + y.
+Proof.
+  intros n x y; constructor.
+  - apply (cantor_pairing_is_injective n x y).
+  - intros H; subst; rewrite (cantor_pairing_is_surjective x y); reflexivity.
+Qed.
+
 Lemma forallb_true_iff {A : Type} (f : A -> bool) :
   forall xs : list A,
   forallb f xs = true <-> (forall x : A, In x xs -> f x = true).
@@ -19,18 +130,14 @@ Proof.
     + tauto.
   - simpl; rewrite andb_true_iff; constructor.
     + intros H; destruct H as [H H0]; intros x H1; destruct H1.
-      { subst; apply H.
-      }
-      { apply IHxs.
-        - apply H0.
-        - apply H1.
-      }
+      * subst; apply H.
+      * apply IHxs.
+        apply H0.
+        apply H1.
     + intros H; constructor.
-      { apply H; left; reflexivity.
-      }
-      { apply IHxs.
+      * apply H; left; reflexivity.
+      * apply IHxs.
         intros x H0; apply H; right; apply H0.
-      }
 Qed.
 
 Definition fold_right_max_0 : list nat -> nat :=
@@ -47,11 +154,7 @@ Proof.
   - simpl; lia.
   - simpl; intros n H; destruct H.
     + lia.
-    + assert (fold_right max 0 ns >= n).
-      { apply IHns.
-        apply H.
-      }
-      lia.
+    + assert (fold_right max 0 ns >= n) by (apply IHns; apply H); lia.
 Qed.
 
 Lemma fold_right_max_0_app :
@@ -145,7 +248,7 @@ Section Chapter1.
 
 Class GoedelianLanguage (mathcalE : Type) : Type :=
   { enum_mathcalE : nat -> mathcalE
-  ; mathcalE_is_enumerable : forall E : mathcalE, {n : nat | enum_mathcalE n = E}
+  ; mathcalE_is_denumerable : forall E : mathcalE, {n : nat | enum_mathcalE n = E}
   ; isSentence : ensemble mathcalE
   ; isProvable : ensemble mathcalE
   ; isRefutable : ensemble mathcalE
@@ -160,7 +263,7 @@ Class GoedelianLanguage (mathcalE : Type) : Type :=
 .
 
 Definition diagonalizer (mathcalE : Type) `{mathcalE_is_goedelian : GoedelianLanguage mathcalE} : nat -> nat :=
-  fun n : nat => proj1_sig (mathcalE_is_enumerable (apply_nat (enum_mathcalE n) n))
+  fun n : nat => proj1_sig (mathcalE_is_denumerable (apply_nat (enum_mathcalE n) n))
 .
 
 Lemma diagonalizer_diagonalizes (mathcalE : Type) `{mathcalE_is_goedelian : GoedelianLanguage mathcalE} :
@@ -169,7 +272,7 @@ Lemma diagonalizer_diagonalizes (mathcalE : Type) `{mathcalE_is_goedelian : Goed
   enum_mathcalE n = E ->
   enum_mathcalE (diagonalizer mathcalE n) = apply_nat E n.
 Proof.
-  intros n E H; unfold diagonalizer; subst; destruct (mathcalE_is_enumerable (apply_nat (enum_mathcalE n) n)) as [d_n]; simpl; tauto.
+  intros n E H; unfold diagonalizer; subst; destruct (mathcalE_is_denumerable (apply_nat (enum_mathcalE n) n)) as [d_n]; simpl; tauto.
 Qed.
 
 Definition expressPredicate (mathcalE : Type) `{mathcalE_is_goedelian : GoedelianLanguage mathcalE} : mathcalE -> ensemble nat -> Prop :=
@@ -206,7 +309,7 @@ Theorem After_Goedel_with_shades_of_Tarski (mathcalE : Type) `{mathcalE_is_goede
 Proof.
   intros mathcalE_is_correct StarOf_complement_P_is_expressible.
   destruct StarOf_complement_P_is_expressible as [H H_express_StarOf_complement_P].
-  destruct (mathcalE_is_enumerable H) as [n n_is_the_goedel_number_of_H].
+  destruct (mathcalE_is_denumerable H) as [n n_is_the_goedel_number_of_H].
   assert (diagonalization_of_n_is_true_iff_n_is_in_StarOf_complement_of_P : isTrue (enum_mathcalE (diagonalizer mathcalE n)) <-> member n (StarOf mathcalE (completement (P mathcalE)))).
   { unfold expressPredicate in H_express_StarOf_complement_P.
     rewrite (diagonalizer_diagonalizes mathcalE n H n_is_the_goedel_number_of_H).
@@ -215,610 +318,118 @@ Proof.
   assert (n_in_StarOf_complement_of_P_iff_diagonalization_of_n_is_not_Provable : member n (StarOf mathcalE (completement (P mathcalE))) <-> ~ isProvable (enum_mathcalE (diagonalizer mathcalE n))).
   { constructor.
     - intros n_in_StarOf_complement_of_P diagonalization_of_n_is_not_Provable.
-      inversion n_in_StarOf_complement_of_P as [A n' diagonalization_of_n_is_in_A A_is_complement_of_P n_is_n']; subst n'.
-      contradiction diagonalization_of_n_is_in_A.
-      apply InP.
-      apply diagonalization_of_n_is_not_Provable.
-    - intros diagonalization_of_n_is_not_Provable.
-      apply InStarOf.
-      intros diagonalization_of_n_is_in_P.
-      contradiction diagonalization_of_n_is_not_Provable.
-      inversion diagonalization_of_n_is_in_P as [n' diagonalization_of_n_is_Provable n_is_n']; subst n'.
-      apply diagonalization_of_n_is_Provable.
+      inversion n_in_StarOf_complement_of_P as [A n' diagonalization_of_n_is_in_A A_is_complement_of_P n_is_n']; subst n'; contradiction diagonalization_of_n_is_in_A.
+      apply InP; apply diagonalization_of_n_is_not_Provable.
+    - intros diagonalization_of_n_is_not_Provable; apply InStarOf.
+      intros diagonalization_of_n_is_in_P; contradiction diagonalization_of_n_is_not_Provable.
+      inversion diagonalization_of_n_is_in_P as [n' diagonalization_of_n_is_Provable n_is_n']; subst n'; apply diagonalization_of_n_is_Provable.
   }
   assert (diagonalization_of_n_is_not_Provable : ~ isProvable (enum_mathcalE (diagonalizer mathcalE n))).
   { intros diagonalization_of_n_is_Provable.
     destruct mathcalE_is_correct as [Provable_implies_true Refutable_implies_false].
-    assert (diagonalization_of_n_is_True : isTrue (enum_mathcalE (diagonalizer mathcalE n))).
-    { apply Provable_implies_true.
-      apply diagonalization_of_n_is_Provable.
-    }
+    assert (diagonalization_of_n_is_True : isTrue (enum_mathcalE (diagonalizer mathcalE n))) by (apply Provable_implies_true; apply diagonalization_of_n_is_Provable).
     tauto.
   }
   exists (enum_mathcalE (diagonalizer mathcalE n)).
   tauto.
 Qed.
 
+Definition the_first_goal (mathcalE : Type) `{mathcalE_is_goedelian : GoedelianLanguage mathcalE} : Prop :=
+  forall A : ensemble nat, is_expressible mathcalE A -> is_expressible mathcalE (StarOf mathcalE A)
+.
+
+Definition the_second_goal (mathcalE : Type) `{mathcalE_is_goedelian : GoedelianLanguage mathcalE} : Prop :=
+  forall A : ensemble nat, is_expressible mathcalE A -> is_expressible mathcalE (completement A)
+.
+
+Definition the_third_goal (mathcalE : Type) `{mathcalE_is_goedelian : GoedelianLanguage mathcalE} : Prop :=
+  is_expressible mathcalE (P mathcalE)
+.
+
+Definition isGoedelSentence (mathcalE : Type) `{mathcalE_is_goedelian : GoedelianLanguage mathcalE} : mathcalE -> ensemble nat -> Prop :=
+  fun E : mathcalE => fun A : ensemble nat => exists n : nat, enum_mathcalE n = E /\ (isTrue E <-> member n A)
+.
+
+Lemma A_Diagonal_Lemma_a (mathcalE : Type) `{mathcalE_is_goedelian : GoedelianLanguage mathcalE} :
+  forall A : ensemble nat,
+  is_expressible mathcalE (StarOf mathcalE A) ->
+  exists E : mathcalE, isGoedelSentence mathcalE E A.
+Proof.
+  intros A StarOf_A_is_expressible; destruct StarOf_A_is_expressible as [H H_express_StarOf_A]; destruct (mathcalE_is_denumerable H) as [n g_H_is_n]; exists (apply_nat H n).
+  assert (isTrue (apply_nat H n) <-> member (diagonalizer mathcalE n) A).
+  { constructor.
+    - intros H_n_is_true; assert (n_is_in_StarOfA : member n (StarOf mathcalE A)) by (apply H_express_StarOf_A; apply H_n_is_true).
+      inversion n_is_in_StarOfA as [A' n' d_n_is_in_A A_is_A' n_is_n']; subst; apply d_n_is_in_A.
+    - intros d_n_is_in_A; apply H_express_StarOf_A; constructor; apply d_n_is_in_A.
+  }
+  assert (enum_mathcalE (diagonalizer mathcalE n) = apply_nat H n).
+  { unfold diagonalizer; rewrite (proj2_sig (mathcalE_is_denumerable (apply_nat (enum_mathcalE n) n))).
+    rewrite g_H_is_n; reflexivity.
+  }
+  exists (diagonalizer mathcalE n); tauto.
+Qed.
+
+Lemma A_Diagonal_Lemma_b (mathcalE : Type) `{mathcalE_is_goedelian : GoedelianLanguage mathcalE} :
+  the_first_goal mathcalE ->
+  forall A : ensemble nat,
+  is_expressible mathcalE A ->
+  exists E : mathcalE, isGoedelSentence mathcalE E A.
+Proof.
+  intros the_first_goal_holds A A_is_expressible; apply A_Diagonal_Lemma_a; apply the_first_goal_holds; apply A_is_expressible.
+Qed.
+
+Inductive T (mathcalE : Type) `{mathcalE_is_goedelian : GoedelianLanguage mathcalE} : ensemble nat :=
+| InT :
+  forall n : nat,
+  isTrue (enum_mathcalE n) ->
+  member n (T mathcalE)
+.
+
+Theorem there_is_no_GoedelSentence_of_complement_of_T (mathcalE : Type) `{mathcalE_is_goedelian : GoedelianLanguage mathcalE} :
+  ~ exists E : mathcalE, isGoedelSentence mathcalE E (completement (T mathcalE)).
+Proof.
+  intros there_is_GoedelSentence_of_complement_of_T.
+  destruct there_is_GoedelSentence_of_complement_of_T as [E E_is_GoedelSentence_of_complement_of_T].
+  destruct E_is_GoedelSentence_of_complement_of_T as [n n_is_g_E_and_E_is_true_iff_n_is_in_complement_T].
+  destruct n_is_g_E_and_E_is_true_iff_n_is_in_complement_T as [n_is_g_E E_is_true_iff_n_is_in_complement_T].
+  assert (E_is_true_iff_n_is_not_in_T : isTrue E <-> ~ member n (T mathcalE)) by (rewrite E_is_true_iff_n_is_in_complement_T; unfold completement; unfold member; reflexivity).
+  assert (E_is_true_iff_n_is_in_T : isTrue E <-> member n (T mathcalE)).
+  { constructor.
+    - intros E_is_true; constructor; rewrite n_is_g_E; apply E_is_true.
+    - intros n_is_inT; inversion n_is_inT as [n' E_is_true n_is_n']; subst n'; rewrite <- n_is_g_E; apply E_is_true.
+  }
+  tauto.
+Qed.
+
+Theorem After_Tarski_1 (mathcalE : Type) `{mathcalE_is_goedelian : GoedelianLanguage mathcalE} :
+  ~ is_expressible mathcalE (StarOf mathcalE (completement (T mathcalE))).
+Proof.
+  intros StarOf_T_is_expressible.
+  destruct (A_Diagonal_Lemma_a mathcalE (completement (T mathcalE)) StarOf_T_is_expressible) as [H H_is_GoedelSentence_for_complement_of_T].
+  contradiction (there_is_no_GoedelSentence_of_complement_of_T mathcalE).
+  exists H; apply H_is_GoedelSentence_for_complement_of_T.
+Qed.
+
+Theorem After_Tarski_2 (mathcalE : Type) `{mathcalE_is_goedelian : GoedelianLanguage mathcalE} :
+  the_first_goal mathcalE ->
+  ~ is_expressible mathcalE (completement (T mathcalE)).
+Proof.
+  intros the_first_goal_holds completement_of_T_is_expressible.
+  apply (After_Tarski_1 mathcalE); apply the_first_goal_holds; apply completement_of_T_is_expressible.
+Qed.
+
+Theorem After_Tarski_3 (mathcalE : Type) `{mathcalE_is_goedelian : GoedelianLanguage mathcalE} :
+  the_first_goal mathcalE ->
+  the_second_goal mathcalE ->
+  ~ is_expressible mathcalE (T mathcalE).
+Proof.
+  intros the_first_goal_holds the_second_goal_holds T_is_expressible.
+  apply (After_Tarski_2 mathcalE the_first_goal_holds); apply the_second_goal_holds; apply T_is_expressible.
+Qed.
+
 End Chapter1.
 
 Section Chapter2.
-
-Definition vr : Set :=
-  nat
-.
-
-Inductive tm : Set :=
-| ivar_tm : vr -> tm
-| zero_tm : tm
-| succ_tm : tm -> tm
-| plus_tm : tm -> tm -> tm
-| mult_tm : tm -> tm -> tm
-| expo_tm : tm -> tm -> tm
-.
-
-Inductive form : Set :=
-| eqn_form : tm -> tm -> form
-| leq_form : tm -> tm -> form
-| neg_form : form -> form
-| imp_form : form -> form -> form
-| all_form : vr -> form -> form
-.
-
-Lemma vr_eq_dec :
-  forall x1 : vr,
-  forall x2 : vr,
-  {x1 = x2} + {x1 <> x2}.
-Proof.
-  apply Nat.eq_dec.
-Qed.
-
-Fixpoint occursFreeIn_tm (z : vr) (t : tm) : bool :=
-  match t with
-  | ivar_tm x => if vr_eq_dec z x then true else false
-  | zero_tm => false
-  | succ_tm t1 => occursFreeIn_tm z t1
-  | plus_tm t1 t2 => occursFreeIn_tm z t1 || occursFreeIn_tm z t2
-  | mult_tm t1 t2 => occursFreeIn_tm z t1 || occursFreeIn_tm z t2
-  | expo_tm t1 t2 => occursFreeIn_tm z t1 || occursFreeIn_tm z t2
-  end
-.
-
-Fixpoint occursFreeIn_form (z : vr) (f : form) : bool :=
-  match f with
-  | eqn_form t1 t2 => occursFreeIn_tm z t1 || occursFreeIn_tm z t2
-  | leq_form t1 t2 => occursFreeIn_tm z t1 || occursFreeIn_tm z t2
-  | neg_form f1 => occursFreeIn_form z f1
-  | imp_form f1 f2 => occursFreeIn_form z f1 || occursFreeIn_form z f2
-  | all_form x f1 => if vr_eq_dec z x then false else occursFreeIn_form z f1
-  end
-.
-
-Fixpoint getFreeVars_tm (t : tm) : list vr :=
-  match t with
-  | ivar_tm x => [x]
-  | zero_tm => []
-  | succ_tm t1 => getFreeVars_tm t1
-  | plus_tm t1 t2 => getFreeVars_tm t1 ++ getFreeVars_tm t2
-  | mult_tm t1 t2 => getFreeVars_tm t1 ++ getFreeVars_tm t2
-  | expo_tm t1 t2 => getFreeVars_tm t1 ++ getFreeVars_tm t2
-  end
-.
-
-Theorem the_rule_of_getFreeVars_tm :
-  forall t : tm,
-  forall x : vr,
-  In x (getFreeVars_tm t) <-> occursFreeIn_tm x t = true.
-Proof.
-  intros t; induction t.
-  - intros vr; simpl; constructor.
-    + intros H; destruct H.
-      { subst.
-        destruct (vr_eq_dec vr vr).
-        - reflexivity.
-        - contradiction.
-      }
-      { contradiction.
-      }
-    + intros H; destruct (vr_eq_dec vr v).
-      { rewrite e; left; reflexivity.
-      }
-      { inversion H.
-      }
-  - intros vr; simpl; constructor.
-    + tauto.
-    + intros H; inversion H.
-  - intros vr; simpl; apply IHt.
-  - intros vr; simpl; rewrite orb_true_iff; rewrite in_app_iff; rewrite IHt1; rewrite IHt2; reflexivity.
-  - intros vr; simpl; rewrite orb_true_iff; rewrite in_app_iff; rewrite IHt1; rewrite IHt2; reflexivity.
-  - intros vr; simpl; rewrite orb_true_iff; rewrite in_app_iff; rewrite IHt1; rewrite IHt2; reflexivity.
-Qed.
-
-Fixpoint getFreeVars_form (f : form) : list vr :=
-  match f with
-  | eqn_form t1 t2 => getFreeVars_tm t1 ++ getFreeVars_tm t2
-  | leq_form t1 t2 => getFreeVars_tm t1 ++ getFreeVars_tm t2
-  | neg_form f1 => getFreeVars_form f1
-  | imp_form f1 f2 => getFreeVars_form f1 ++ getFreeVars_form f2
-  | all_form x f1 => remove vr_eq_dec x (getFreeVars_form f1)
-  end
-.
-
-Theorem the_rule_of_getFreeVars_form :
-  forall f : form,
-  forall x : vr,
-  In x (getFreeVars_form f) <-> occursFreeIn_form x f = true.
-Proof.
-  intros f; induction f.
-  - intros vr; simpl; rewrite orb_true_iff; rewrite in_app_iff; rewrite the_rule_of_getFreeVars_tm; rewrite the_rule_of_getFreeVars_tm; reflexivity.
-  - intros vr; simpl; rewrite orb_true_iff; rewrite in_app_iff; rewrite the_rule_of_getFreeVars_tm; rewrite the_rule_of_getFreeVars_tm; reflexivity.
-  - intros vr; simpl; apply IHf.
-  - intros vr; simpl; rewrite orb_true_iff; rewrite in_app_iff; rewrite IHf1; rewrite IHf2; reflexivity.
-  - intros vr; simpl; constructor.
-    + intros H.
-      assert (In vr (getFreeVars_form f) /\ vr <> v).
-      { apply (in_remove vr_eq_dec (getFreeVars_form f) vr v); apply H.
-      }
-      destruct H0 as [H0 H1]; destruct (vr_eq_dec vr v).
-      { contradiction H1.
-      }
-      { apply IHf; apply H0.
-      }
-    + intros H; destruct (vr_eq_dec vr v).
-      { inversion H.
-      }
-      { apply in_in_remove.
-        - apply n.
-        - apply IHf; apply H.
-      }
-Qed.
-
-Definition value_of_N : Set :=
-  nat
-.
-
-Definition value_assignment : Set :=
-  vr -> value_of_N
-.
-
-Fixpoint eval_tm (va : value_assignment) (t : tm) : value_of_N :=
-  match t with
-  | ivar_tm x => va x
-  | zero_tm => 0
-  | succ_tm t1 => S (eval_tm va t1)
-  | plus_tm t1 t2 => eval_tm va t1 + eval_tm va t2
-  | mult_tm t1 t2 => eval_tm va t1 * eval_tm va t2
-  | expo_tm t1 t2 => (eval_tm va t1)^(eval_tm va t2)
-  end
-.
-
-Lemma eval_tm_extensionality :
-  forall t : tm,
-  forall va1 : value_assignment,
-  forall va2 : value_assignment,
-  (forall x : vr, occursFreeIn_tm x t = true -> va1 x = va2 x) ->
-  eval_tm va1 t = eval_tm va2 t.
-Proof.
-  intros t; induction t.
-  - simpl; intros va1 va2 H; apply H; destruct (vr_eq_dec v v).
-    + reflexivity.
-    + contradiction.
-  - simpl; intros va1 va2 H.
-    reflexivity.
-  - simpl; intros va1 va2 H.
-    rewrite (IHt va1 va2).
-    reflexivity.
-    apply H.
-  - simpl; intros va1 va2 H.
-    rewrite (IHt1 va1 va2).
-    rewrite (IHt2 va1 va2).
-    reflexivity.
-    intros x H0; apply H; apply orb_true_iff; tauto.
-    intros x H0; apply H; apply orb_true_iff; tauto.
-  - simpl; intros va1 va2 H.
-    rewrite (IHt1 va1 va2).
-    rewrite (IHt2 va1 va2).
-    reflexivity.
-    intros x H0; apply H; apply orb_true_iff; tauto.
-    intros x H0; apply H; apply orb_true_iff; tauto.
-  - simpl; intros va1 va2 H.
-    rewrite (IHt1 va1 va2).
-    rewrite (IHt2 va1 va2).
-    reflexivity.
-    intros x H0; apply H; apply orb_true_iff; tauto.
-    intros x H0; apply H; apply orb_true_iff; tauto.
-Qed.
-
-Fixpoint eval_form (va : value_assignment) (f : form) : Prop :=
-  match f with
-  | eqn_form t1 t2 => eval_tm va t1 = eval_tm va t2
-  | leq_form t1 t2 => eval_tm va t1 <= eval_tm va t2
-  | neg_form f1 => ~ eval_form va f1
-  | imp_form f1 f2 => eval_form va f1 -> eval_form va f2
-  | all_form x f1 => forall val : value_of_N, eval_form (fun z : vr => if vr_eq_dec x z then val else va z) f1
-  end
-.
-
-Lemma eval_form_extensionality :
-  forall f : form,
-  forall va1 : value_assignment,
-  forall va2 : value_assignment,
-  (forall x : vr, occursFreeIn_form x f = true -> va1 x = va2 x) ->
-  eval_form va1 f <-> eval_form va2 f.
-Proof.
-  intros f; induction f.
-  - simpl; intros va1 va2 H.
-    rewrite (eval_tm_extensionality t va1 va2).
-    rewrite (eval_tm_extensionality t0 va1 va2).
-    reflexivity.
-    intros x H0; apply H; apply orb_true_iff; tauto.
-    intros x H0; apply H; apply orb_true_iff; tauto.
-  - simpl; intros va1 va2 H.
-    rewrite (eval_tm_extensionality t va1 va2).
-    rewrite (eval_tm_extensionality t0 va1 va2).
-    reflexivity.
-    intros x H0; apply H; apply orb_true_iff; tauto.
-    intros x H0; apply H; apply orb_true_iff; tauto.
-  - simpl; intros va1 va2 H.
-    rewrite (IHf va1 va2).
-    reflexivity.
-    intros x H0; apply H; tauto.
-  - simpl; intros va1 va2 H.
-    rewrite (IHf1 va1 va2).
-    rewrite (IHf2 va1 va2).
-    reflexivity.
-    intros x H0; apply H; apply orb_true_iff; tauto.
-    intros x H0; apply H; apply orb_true_iff; tauto.
-  - simpl; intros va1 va2 H.
-    cut (
-      forall n : value_of_N,
-      eval_form (fun z : vr => if vr_eq_dec v z then n else va1 z) f <->  eval_form (fun z : vr => if vr_eq_dec v z then n else va2 z) f
-    ).
-    { constructor.
-      - intros H1 n; apply H0; apply H1.
-      - intros H1 n; apply H0; apply H1.
-    }
-    intros n.
-    rewrite (IHf (fun z : vr => if vr_eq_dec v z then n else va1 z) (fun z : vr => if vr_eq_dec v z then n else va2 z)).
-    reflexivity.
-    intros x H0; destruct (vr_eq_dec v x).
-    { reflexivity.
-    }
-    { apply H.
-      destruct (vr_eq_dec x v).
-      - contradiction n0; rewrite e; reflexivity.
-      - apply H0.
-    }
-Qed.
-
-Fixpoint make_numeral (n : value_of_N) : tm :=
-  match n with
-  | 0 => zero_tm
-  | S n' => succ_tm (make_numeral n')
-  end
-.
-
-Lemma eval_tm_make_numeral :
-  forall n : value_of_N,
-  forall va : value_assignment,
-  eval_tm va (make_numeral n) = n.
-Proof.
-  intros n; induction n.
-  - simpl; intros va; reflexivity.
-  - simpl; intros va; rewrite IHn; reflexivity.
-Qed.
-
-Definition substitution : Set :=
-  list (vr * tm)
-.
-
-Fixpoint substitute_vr (sigma : substitution) (x : vr) : tm :=
-  match sigma with
-  | [] => ivar_tm x
-  | (x1, tm1) :: sigma' => if vr_eq_dec x x1 then tm1 else substitute_vr sigma' x
-  end
-.
-
-Fixpoint substitute_tm (sigma : substitution) (t : tm) : tm :=
-  match t with
-  | ivar_tm x => substitute_vr sigma x
-  | zero_tm => zero_tm
-  | succ_tm t1 => succ_tm (substitute_tm sigma t1)
-  | plus_tm t1 t2 => plus_tm (substitute_tm sigma t1) (substitute_tm sigma t2)
-  | mult_tm t1 t2 => mult_tm (substitute_tm sigma t1) (substitute_tm sigma t2)
-  | expo_tm t1 t2 => expo_tm (substitute_tm sigma t1) (substitute_tm sigma t2)
-  end
-.
-
-Theorem substitute_tm_preserves_eval_tm :
-  forall t : tm,
-  forall sigma : substitution,
-  forall va : value_assignment,
-  eval_tm (fun z : vr => eval_tm va (substitute_vr sigma z)) t = eval_tm va (substitute_tm sigma t).
-Proof.
-  intros t; induction t.
-  - intros sigma va; simpl; reflexivity.
-  - intros sigma va; simpl; reflexivity.
-  - intros sigma va; simpl; rewrite IHt; reflexivity.
-  - intros sigma va; simpl; rewrite IHt1; rewrite IHt2; reflexivity.
-  - intros sigma va; simpl; rewrite IHt1; rewrite IHt2; reflexivity.
-  - intros sigma va; simpl; rewrite IHt1; rewrite IHt2; reflexivity.
-Qed.
-
-Definition getMaxNumOfFreeVars_tm (t : tm) : vr :=
-  fold_right_max_0 (getFreeVars_tm t)
-.
-
-Lemma getMaxNumOfFreeVars_tm_lt :
-  forall t : tm,
-  forall x : vr,
-  getMaxNumOfFreeVars_tm t < x ->
-  occursFreeIn_tm x t = false.
-Proof.
-  unfold getMaxNumOfFreeVars_tm; intros t; induction t.
-  - simpl; intros x H; destruct (vr_eq_dec x v).
-    + lia.
-    + reflexivity.
-  - simpl; intros x H; tauto.
-  - simpl; intros x H; apply IHt; apply H.
-  - simpl; intros x H; apply orb_false_iff; rewrite fold_right_max_0_app in H; constructor.
-    + apply IHt1; lia.
-    + apply IHt2; lia.
-  - simpl; intros x H; apply orb_false_iff; rewrite fold_right_max_0_app in H; constructor.
-    + apply IHt1; lia.
-    + apply IHt2; lia.
-  - simpl; intros x H; apply orb_false_iff; rewrite fold_right_max_0_app in H; constructor.
-    + apply IHt1; lia.
-    + apply IHt2; lia.
-Qed.
-
-Definition isFreshVarIn_substitute_tm (sigma : substitution) (z : vr) (t : tm) : Prop :=
-  forallb (fun x : vr => negb (occursFreeIn_tm z (substitute_vr sigma x))) (getFreeVars_tm t) = true
-.
-
-Definition isFreshVarIn_substitute_form (sigma : substitution) (z : vr) (f : form) : Prop :=
-  forallb (fun x : vr => negb (occursFreeIn_tm z (substitute_vr sigma x))) (getFreeVars_form f) = true
-.
-
-Definition chi (sigma : substitution) (f : form) : vr :=
-  S (fold_right_max_0 (map (fun x : vr => getMaxNumOfFreeVars_tm (substitute_vr sigma x)) (getFreeVars_form f)))
-.
-
-Theorem the_rule_of_chi :
-  forall f : form,
-  forall sigma : substitution,
-  isFreshVarIn_substitute_form sigma (chi sigma f) f.
-Proof.
-  assert ( claim1 :
-    forall sigma : substitution,
-    forall f : form,
-    forall x : vr,
-    occursFreeIn_form x f = true ->
-    occursFreeIn_tm (chi sigma f) (substitute_vr sigma x) = false
-  ).
-  { intros sigma f x H.
-    assert (getMaxNumOfFreeVars_tm (substitute_vr sigma x) < chi sigma f).
-    { unfold chi; unfold fold_right_max_0.
-      cut (fold_right max 0 (map (fun z : vr => getMaxNumOfFreeVars_tm (substitute_vr sigma z)) (getFreeVars_form f)) >= getMaxNumOfFreeVars_tm (substitute_vr sigma x)).
-      { lia.
-      }
-      rewrite <- the_rule_of_getFreeVars_form in H.
-      apply fold_right_max_0_in; apply in_map_iff.
-      exists x; constructor.
-      - reflexivity.
-      - apply H.
-    }
-    apply getMaxNumOfFreeVars_tm_lt; apply H0.
-  }
-  unfold isFreshVarIn_substitute_form; intros f sigma; apply forallb_true_iff.
-  intros x H; apply negb_true_iff; apply claim1; apply the_rule_of_getFreeVars_form; apply H.
-Qed.
-
-Fixpoint substitute_form (sigma : substitution) (f : form) : form :=
-  match f with
-  | eqn_form t1 t2 => eqn_form (substitute_tm sigma t1) (substitute_tm sigma t2)
-  | leq_form t1 t2 => leq_form (substitute_tm sigma t1) (substitute_tm sigma t2)
-  | neg_form f1 => neg_form (substitute_form sigma f1)
-  | imp_form f1 f2 => imp_form (substitute_form sigma f1) (substitute_form sigma f2)
-  | all_form x f1 =>
-    let z : vr := chi sigma f in
-    all_form z (substitute_form ((x, ivar_tm z) :: sigma) f1)
-  end
-.
-
-Theorem substitute_form_preserves_eval_form :
-  forall f : form,
-  forall sigma : substitution,
-  forall va : value_assignment,
-  eval_form (fun z : vr => eval_tm va (substitute_vr sigma z)) f <-> eval_form va (substitute_form sigma f).
-Proof.
-  intros f; induction f.
-  - intros sigma va; simpl.
-    rewrite substitute_tm_preserves_eval_tm; rewrite substitute_tm_preserves_eval_tm; reflexivity.
-  - intros sigma va; simpl.
-    rewrite substitute_tm_preserves_eval_tm; rewrite substitute_tm_preserves_eval_tm; reflexivity.
-  - intros sigma va; simpl.
-    rewrite IHf; reflexivity.
-  - intros sigma va; simpl.
-    rewrite IHf1; rewrite IHf2; reflexivity.
-  - intros sigma va. simpl.
-    cut (
-      forall n : value_of_N,
-      eval_form (fun z : vr => if vr_eq_dec v z then n else eval_tm va (substitute_vr sigma z)) f <-> eval_form (fun z : vr => if vr_eq_dec (chi sigma (all_form v f)) z then n else va z) (substitute_form ((v, ivar_tm (chi sigma (all_form v f))) :: sigma) f)
-    ).
-    { intros H; constructor.
-      - intros H0 n; apply H; apply H0.
-      - intros H0 n; apply H; apply H0.
-    }
-    intros n; rewrite <- (IHf ((v, ivar_tm (chi sigma (all_form v f))) :: sigma) (fun z : vr => if vr_eq_dec (chi sigma (all_form v f)) z then n else va z)); apply eval_form_extensionality.
-    intros x H; simpl; destruct (vr_eq_dec v x).
-    { destruct (vr_eq_dec x v).
-      - simpl; destruct (vr_eq_dec (chi sigma (all_form v f)) (chi sigma (all_form v f))).
-        + reflexivity.
-        + contradiction.
-      - contradiction n0; rewrite e; reflexivity.
-    }
-    { destruct (vr_eq_dec x v).
-      - contradiction n0; rewrite e; reflexivity.
-      - apply eval_tm_extensionality.
-        intros x' H0; destruct (vr_eq_dec (chi sigma (all_form v f)) x').
-        + subst.
-          assert (isFreshVarIn_substitute_form sigma (chi sigma (all_form v f)) (all_form v f)).
-            apply the_rule_of_chi.
-          unfold isFreshVarIn_substitute_form in H1; rewrite forallb_true_iff in H1.
-          assert (negb (occursFreeIn_tm (chi sigma (all_form v f)) (substitute_vr sigma x)) = true).
-          { apply H1; apply the_rule_of_getFreeVars_form; simpl; destruct (vr_eq_dec x v).
-            - contradiction.
-            - tauto. 
-          }
-          rewrite H0 in H2; inversion H2.
-        + reflexivity.
-    }
-Qed.
-
-Lemma substitute_tm_make_numeral :
-  forall n : value_of_N,
-  forall sigma : substitution,
-  substitute_tm sigma (make_numeral n) = make_numeral n.
-Proof.
-  intros n; induction n.
-  - intros sigma; simpl; reflexivity.
-  - intros sigma; simpl; rewrite (IHn sigma); reflexivity.
-Qed.
-
-Ltac simpl_eval_tm_make_numeral := repeat (rewrite substitute_tm_make_numeral); repeat (rewrite eval_tm_make_numeral).
-
-Ltac simpl_in_eval_tm_make_numeral H := repeat (rewrite substitute_tm_make_numeral in H); repeat (rewrite eval_tm_make_numeral in H).
-
-Lemma occursFreeIn_tm_make_numeral :
-  forall val : value_of_N,
-  forall x : vr,
-  occursFreeIn_tm x (make_numeral val) = false.
-Proof.
-  intros val; induction val.
-  - intros x; simpl; reflexivity.
-  - intros x; simpl; rewrite (IHval x); reflexivity.
-Qed.
-
-Ltac simplify_make_numeral := repeat (rewrite substitute_tm_make_numeral); repeat (apply occursFreeIn_tm_make_numeral).
-
-Lemma vr_eq_dec_is_Nat_eq_dec {A : Type} :
-  forall x1 : A,
-  forall x2 : A,
-  forall z1 : vr,
-  forall z2 : vr,
-  (if vr_eq_dec z1 z2 then x1 else x2) = (if Nat.eq_dec z1 z2 then x1 else x2).
-Proof.
-  intros x1 x2 z1 z2.
-  destruct (vr_eq_dec z1 z2).
-  - destruct (Nat.eq_dec z1 z2).
-    + reflexivity.
-    + contradiction.
-  - destruct (Nat.eq_dec z1 z2).
-    + contradiction.
-    + reflexivity.
-Qed.
-
-Ltac eval_vr_eq_dec := repeat (rewrite vr_eq_dec_is_Nat_eq_dec; simpl).
-
-Ltac eval_in_vr_eq_dec H := repeat (rewrite vr_eq_dec_is_Nat_eq_dec in H; simpl in H).
-
-Ltac auto_show_it_is_sentence := tryif (apply orb_false_iff; constructor) then auto_show_it_is_sentence else (eval_vr_eq_dec; simplify_make_numeral).
-
-Fixpoint relation_of_arity (n : nat) : Type :=
-  match n with
-  | 0 => Prop
-  | S n' => value_of_N -> relation_of_arity n'
-  end
-.
-
-Fixpoint lift_relation (n : nat) : relation_of_arity (S n) -> nat -> relation_of_arity n :=
-  match n as n0 return relation_of_arity (S n0) -> nat -> relation_of_arity n0 with
-  | 0 =>
-    fun pred : value_of_N -> Prop =>
-    fun val : value_of_N =>
-    pred val
-  | S n' =>
-    fun pred : value_of_N -> value_of_N -> relation_of_arity n' =>
-    fun val : value_of_N =>
-    fun val' : value_of_N =>
-    lift_relation n' (pred val') val 
-  end
-.
-
-Fixpoint express_relation (n : nat) : form -> relation_of_arity n -> Prop :=
-  match n as n0 return form -> relation_of_arity n0 -> Prop with
-  | 0 =>
-    fun f : form =>
-    fun pred : Prop =>
-    (forall x : vr, occursFreeIn_form x f = false) /\ (pred <-> forall va : value_assignment, eval_form va f)
-  | S n' =>
-    fun f : form =>
-    fun pred : value_of_N -> relation_of_arity n' =>
-    forall val : value_of_N, express_relation n' (substitute_form [(n', make_numeral val)] f) (lift_relation n' pred val)
-  end
-.
-
-Example express_relation_example1 :
-  express_relation 2 (leq_form (ivar_tm 0) (ivar_tm 1)) (fun x0 : value_of_N => fun x1 : value_of_N => x0 <= x1).
-Proof.
-  simpl; intros val1 val0; constructor.
-  - intros x; auto_show_it_is_sentence.
-  - constructor.
-    + intros H va.
-      eval_vr_eq_dec; simpl_eval_tm_make_numeral; tauto.
-    + intros H.
-      assert (H0 := H (fun _ : vr => 0)).
-      eval_in_vr_eq_dec H0; simpl_in_eval_tm_make_numeral H0; tauto.
-Qed.
-
-Fixpoint function_of_arity (n : nat) : Type :=
-  match n with
-  | 0 => value_of_N
-  | S n' => value_of_N -> function_of_arity n'
-  end
-.
-
-Fixpoint lift_function (n : nat) : function_of_arity (S n) -> nat -> function_of_arity n :=
-  match n as n0 return function_of_arity (S n0) -> nat -> function_of_arity n0 with
-  | 0 =>
-    fun func : value_of_N -> value_of_N =>
-    fun val : value_of_N =>
-    func val
-  | S n' =>
-    fun func : value_of_N -> value_of_N -> function_of_arity n' =>
-    fun val : value_of_N =>
-    fun val' : value_of_N =>
-    lift_function n' (func val') val 
-  end
-.
-
-Fixpoint express_function (n : nat) : form -> function_of_arity n -> Prop :=
-  match n as n0 return form -> function_of_arity n0 -> Prop with
-  | 0 =>
-    fun f : form =>
-    fun func : value_of_N =>
-    forall val : value_of_N,
-    let f' : form := substitute_form [(0, make_numeral val)] f in
-    (forall x : vr, occursFreeIn_form x f' = false) /\ (val = func <-> forall va : value_assignment, eval_form va f')
-  | S n' =>
-    fun f : form =>
-    fun func : value_of_N -> function_of_arity n' =>
-    forall val : value_of_N, express_function n' (substitute_form [(n, make_numeral val)] f) (lift_function n' func val)
-  end
-.
-
-Example express_function_example1 :
-  express_function 3 (eqn_form (ivar_tm 0) (plus_tm (ivar_tm 1) (plus_tm (ivar_tm 2) (ivar_tm 3)))) (fun x1 : value_of_N => fun x2 : value_of_N => fun x3 : value_of_N => x1 + (x2 + x3)).
-Proof.
-  simpl; intros val3 val2 val1 val0; constructor.
-  - intros x; auto_show_it_is_sentence.
-  - constructor.
-    + intros H va.
-      eval_vr_eq_dec; simpl_eval_tm_make_numeral; tauto.
-    + intros H.
-      assert (H0 := H (fun _ : vr => 0)).
-      eval_in_vr_eq_dec H0; simpl_in_eval_tm_make_numeral H0; tauto.
-Qed.
 
 End Chapter2.
 
